Move state handling into resolution_prover monad.

prover_state.lean
@@ -8,6 +8,7 @@ structure active_cls :=
 structure resolution_prover_state :=
 (active : rb_map name active_cls)
 (passive : rb_map name cls)
+(newly_derived : list cls)
 
 meta_definition resolution_prover :=
 stateT resolution_prover_state tactic
@@ -16,14 +17,44 @@ attribute [instance]
 meta_definition resolution_prover_is_monad : monad resolution_prover :=
 stateT_is_monad _ _
 
-meta_definition get_active : resolution_prover (rb_map name active_cls) :=
-do state ← stateT.read, return (resolution_prover_state.active state)
-
 meta_definition resolution_prover_of_tactic {a} (tac : tactic a) : resolution_prover a :=
 λs, do res ← tac, return (res, s)
 
+meta_definition resolution_prover.fail {A B : Type} [has_to_format B] (msg : B) : resolution_prover A :=
+resolution_prover_of_tactic (tactic.fail msg)
+
+meta_definition resolution_prover.failed {A : Type} : resolution_prover A :=
+resolution_prover.fail "failed"
+
+meta_definition resolution_prover.orelse {A : Type} (p1 p2 : resolution_prover A) : resolution_prover A :=
+take state, p1 state <|> p2 state
+
+attribute [instance]
+meta_definition resolution_prover_is_alternative : alternative resolution_prover :=
+alternative.mk (@monad.map _ resolution_prover_is_monad)
+  (@applicative.pure _ (monad_is_applicative resolution_prover))
+  (@applicative.seq _ (monad_is_applicative resolution_prover))
+  @resolution_prover.failed
+  @resolution_prover.orelse
+
+meta_definition get_active : resolution_prover (rb_map name active_cls) :=
+do state ← stateT.read, return (resolution_prover_state.active state)
+
+example : resolution_prover (rb_map name active_cls) :=
+@orelse resolution_prover _ _ get_active resolution_prover.failed
+
+meta_definition remove_redundant (n : name) : resolution_prover unit :=
+@monad.bind resolution_prover _ _ _ stateT.read (λstate,
+stateT.write (resolution_prover_state.mk (rb_map.erase (resolution_prover_state.active state) n)
+  (resolution_prover_state.passive state) (resolution_prover_state.newly_derived state)))
+
+meta_definition add_inferred (c : cls) : resolution_prover unit :=
+@monad.bind resolution_prover _ _ _ stateT.read (λstate,
+stateT.write (resolution_prover_state.mk (resolution_prover_state.active state)
+  (resolution_prover_state.passive state) (c :: resolution_prover_state.newly_derived state)))
+
 meta_definition inference :=
-active_cls → resolution_prover (list cls × list name)
+active_cls → resolution_prover unit
 
 meta_definition list_contains {a} [decidable_eq a] (elem : a) (l : list a) : bool :=
 match l with
@@ -31,29 +62,26 @@ match l with
 | nil := ff
 end
 
-meta_definition seq_inferences (infs : list inference) : inference :=
-λgiven, match infs with
-| [] := return ([], [])
-| inf::infs' := do
-    (newly_derived, redundant) ← inf given,
-    if list_contains (active_cls.id given) redundant = tt then
-      return (newly_derived, redundant)
-    else do
-      (newly_derived', redundant') ← seq_inferences infs' given,
-      return (newly_derived ++ newly_derived', redundant ++ redundant')
-end
+meta_definition seq_inferences : list inference → inference
+| [] := λgiven, return ()
+| (inf::infs) := λgiven, do
+    inf given,
+    now_active ← get_active,
+    if rb_map.contains now_active (active_cls.id given) = tt then
+      seq_inferences infs given
+    else
+      return ()
 
 meta_definition redundancy_inference (is_redundant : active_cls → resolution_prover bool) : inference :=
 λgiven, do
 is_red ← is_redundant given,
-return ([], if is_red = tt then [active_cls.id given] else [])
+if is_red = tt then remove_redundant (active_cls.id given) else return ()
 
 meta_definition simp_inference (simpl : active_cls → resolution_prover (option cls)) : inference :=
-λgiven, do
-maybe_simpld ← simpl given,
+λgiven, do maybe_simpld ← simpl given,
 match maybe_simpld with
-| some simpld := return ([simpld], [active_cls.id given])
-| none := return ([], [])
+| some simpld := do add_inferred simpld, remove_redundant (active_cls.id given)
+| none := return ()
 end
 
 meta_definition selection_strategy := cls → resolution_prover (list nat)
@@ -64,4 +92,9 @@ meta_definition dumb_selection : selection_strategy :=
 | neg_lit::_ := [neg_lit]
 end
 
-meta_definition preprocessing_rule := list cls → resolution_prover (list cls)
+meta_definition preprocessing_rule (f : list cls → resolution_prover (list cls)) : resolution_prover unit := do
+state ← stateT.read,
+newly_derived' ← f (resolution_prover_state.newly_derived state),
+@monad.bind resolution_prover _ _ _ stateT.read (λstate',
+stateT.write (resolution_prover_state.mk (resolution_prover_state.active state')
+  (resolution_prover_state.passive state') newly_derived'))
